seems ready to prove FLTR

theories/logrel/logrel_prim.v
@@ -4,10 +4,139 @@ From HypVeri.lang Require Import lang.
 From HypVeri.algebra Require Import base base_extra mem mailbox trans.
 From HypVeri.logrel Require Export logrel logrel_extra big_sepSS.
 
+Section slice.
+  Context `{hypconst:HypervisorConstants}.
+
+  Definition set_of_vmids : gset VMID := (list_to_set list_of_vmids).
+
+  Context `{vmG: !gen_VMG Σ}.
+  Context (Φ : (gmap Addr transaction) -> VMID -> VMID -> iProp Σ).
+  (*TODO*)
+  Definition trans_preserve_except i (trans trans': (gmap Addr transaction)) :=
+    map_Forall (λ h tran, ¬(tran.1.1.1.1 = i ∨ tran.1.1.1.2 = i) -> ∃ tran', trans' !! h = Some tran' ∧ tran = tran') trans.
+
+
+  Definition trans_preserve_slice i j (trans trans': (gmap Addr transaction)):=
+    filter (λ kv, kv.2.1.1.1.1 = i ∧ kv.2.1.1.1.2 = j) trans
+                        = filter (λ kv, kv.2.1.1.1.1 = i ∧ kv.2.1.1.1.2 = j) trans'.
+
+  Definition trans_preserve_only i (trans trans': (gmap Addr transaction)) :=
+    filter (λ kv, kv.2.1.1.1.1 = i ∨ kv.2.1.1.1.2 = i) trans
+                        = filter (λ kv, kv.2.1.1.1.1 = i ∨ kv.2.1.1.1.2 = i) trans'.
+  Definition slice_wf :=
+    ∀ i j trans trans', trans_preserve_slice i j trans trans'->
+    (Φ trans i j ⊣⊢ Φ trans' i j).
+
+  Definition slice_wf2 :=
+    ∀ i j (trans trans' : gmap Addr transaction),
+    dom (gset _) (filter (λ kv, kv.2.1.1.1.1 = i ∧ kv.2.1.1.1.2 = j)%type trans') ⊆ dom _ trans ->
+    ([∗ map] h ↦ tran ∈ trans, h -{1/2}>t tran.1) ⊢
+    (Φ trans' i j) ∗-∗ (Φ (map_zip (fst<$>trans) (snd <$>trans')) i j).
+
+  Class SliceWf :=
+    {
+      valid : slice_wf;
+      agree : slice_wf2
+    }.
+
+  End slice.
+
+  Section vmprop.
+  Context `{HypervisorConstants}.
+  Context `{!HypervisorParameters}.
+  Context (i : VMID).
+  Context `{vmG: !gen_VMG Σ}.
+  Context (Φ : (gmap Addr transaction) -> VMID -> VMID -> iProp Σ).
+
+  Definition vmprop_zero_pre (Ψ: PID -d> PID -d> iPropO Σ) :PID -d> PID -d> iPropO Σ :=
+    λ p_tx p_rx, (∃ trans'',
+                           (* transaction and pagetable entries *)
+                           transaction_hpool_global_transferred trans'' ∗
+                           big_sepSS_singleton set_of_vmids i (Φ trans'') ∗
+                           (* RX *)
+                           rx_page i p_rx ∗ (∃ mem_rx, memory_page p_rx mem_rx) ∗
+                           rx_pages ((list_to_set (list_of_vmids)) ∖ {[i]}) ∗
+                           return_reg_rx i ∗
+                           VMProp i (Ψ p_tx p_rx) (1/2)%Qp)%I.
+
+  Definition vmprop_unknown_pre
+    (Ψ : PID -d> PID -d> iPropO Σ)
+    :PID -d> PID -d> iPropO Σ :=
+    λ p_tx p_rx,
+    (∃ (trans' : gmap Word transaction) rx_state,
+               (* transaction and pagetable entries *)
+               transaction_hpool_global_transferred trans' ∗
+               big_sepSS_singleton set_of_vmids i (Φ trans') ∗
+               R0 @@ V0 ->r encode_hvc_func(Run) ∗ R1 @@ V0 ->r encode_vmid(i) ∗ (∃ r2, R2 @@ V0 ->r r2) ∗
+               (* status of RX *)
+               RX_state@ i := rx_state ∗
+               (* RX *)
+               (rx_page i p_rx) ∗
+               (∃ mem_rx, memory_page p_rx mem_rx) ∗
+               (* rx pages for all other VMs *)
+               rx_pages (list_to_set (list_of_vmids) ∖ {[i]}) ∗
+               (* if i yielding, we give following resources back to pvm *)
+               VMProp V0 (vmprop_zero_pre Ψ p_tx p_rx) (1/2)%Qp)%I.
+
+  Local Instance vmprop_unknown_pre_contractive : Contractive (vmprop_unknown_pre).
+  Proof.
+    rewrite /vmprop_unknown_pre => n vmprop_unknown vmprop_unknown' Hvmprop_unknown p_tx p_rx /=.
+    do 13 f_equiv.
+    rewrite /VMProp /=.
+    do 6 f_equiv.
+    f_contractive.
+    rewrite /vmprop_zero_pre.
+    do 8 f_equiv.
+    rewrite /VMProp.
+    repeat f_equiv.
+  Qed.
+
+  Definition vmprop_unknown:= fixpoint (vmprop_unknown_pre).
+
+  Definition vmprop_zero := vmprop_zero_pre vmprop_unknown.
+
+  Lemma vmprop_unknown_def : vmprop_unknown ≡
+    λ p_tx p_rx,
+      (∃ (trans' : gmap Word transaction) rx_state,
+          transaction_hpool_global_transferred trans' ∗
+          big_sepSS_singleton set_of_vmids i (Φ trans') ∗
+          R0 @@ V0 ->r encode_hvc_func(Run) ∗ R1 @@ V0 ->r encode_vmid(i) ∗ (∃ r2, R2 @@ V0 ->r r2) ∗
+          RX_state@ i := rx_state ∗
+          (rx_page i p_rx) ∗
+          (∃ mem_rx, memory_page p_rx mem_rx) ∗
+          rx_pages (list_to_set (list_of_vmids) ∖ {[i]}) ∗
+          VMProp V0 (vmprop_zero p_tx p_rx) (1/2)%Qp)%I.
+  Proof.
+    rewrite /vmprop_unknown //.
+    rewrite (fixpoint_unfold vmprop_unknown_pre).
+    setoid_reflexivity.
+  Qed.
+
+  Global Instance vmprop_unknown_proper: Proper ((=) ==> (=) ==> (⊣⊢)) vmprop_unknown.
+  Proof. apply _. Qed.
+
+  Lemma vmprop_unknown_eq (p_tx p_rx:PID) : vmprop_unknown p_tx p_rx ⊣⊢
+      (∃ (trans' : gmap Word transaction) rx_state,
+               transaction_hpool_global_transferred trans' ∗
+               big_sepSS_singleton set_of_vmids i (Φ trans') ∗
+               R0 @@ V0 ->r encode_hvc_func(Run) ∗ R1 @@ V0 ->r encode_vmid(i) ∗ (∃ r2, R2 @@ V0 ->r r2) ∗
+               RX_state@ i := rx_state ∗
+               (rx_page i p_rx) ∗
+               (∃ mem_rx, memory_page p_rx mem_rx) ∗
+               rx_pages (list_to_set (list_of_vmids) ∖ {[i]}) ∗
+               VMProp V0 (vmprop_zero p_tx p_rx) (1/2)%Qp)%I.
+    Proof.
+      rewrite /vmprop_unknown.
+      (* be patient, this line takes 30+ sec.. *)
+      apply (fixpoint_unfold vmprop_unknown_pre).
+    Qed.
+
+  End vmprop.
+
 Section logrel_prim.
 
-  Context `{hypconst:HypervisorConstants}.
-  Context `{hypparams:!HypervisorParameters}.
+  Context `{HypervisorConstants}.
+  Context `{!HypervisorParameters}.
   Context `{vmG: !gen_VMG Σ}.
 
   (* Definition trans_rel_primary (i:VMID) (trans trans': gmap Word transaction): Prop := *)
@@ -27,39 +156,16 @@ Section logrel_prim.
   Definition transaction_pagetable_entries_transferred_slice (trans: gmap Addr transaction) (i: VMID) (j: VMID) : iProp Σ :=
     big_sepFM trans (λ kv, (kv.2.1.1.1.1 = i ∧ kv.2.1.1.1.2 = j) ∧ kv.2.1.2 = Donation) (λ k v, k -{1/4}>t v.1 ∗ pgt_1_4 v.1.1.2 v.1.1.1.1 true)%I.
 
-  Definition set_of_vmids : gset VMID := (list_to_set list_of_vmids).
 
-  Definition trans_preserve_slice i j (trans trans': (gmap Addr transaction)):=
-    filter (λ kv, kv.2.1.1.1.1 = i ∧ kv.2.1.1.1.2 = j) trans
-                        = filter (λ kv, kv.2.1.1.1.1 = i ∧ kv.2.1.1.1.2 = j) trans'.
+  Definition slice_transfer_all :=
+    (λ trans i j, transaction_pagetable_entries_transferred_slice trans i j
+                ∗ retrievable_transaction_transferred_slice trans i j
+                ∗ transferred_memory_slice trans i j)%I.
 
-  Definition trans_preserve_only i (trans trans': (gmap Addr transaction)) :=
-    filter (λ kv, kv.2.1.1.1.1 = i ∨ kv.2.1.1.1.2 = i) trans
-                        = filter (λ kv, kv.2.1.1.1.1 = i ∨ kv.2.1.1.1.2 = i) trans'.
-
-  (*TODO*)
-  Definition trans_preserve_except i (trans trans': (gmap Addr transaction)) :=
-    map_Forall (λ h tran, ¬(tran.1.1.1.1 = i ∨ tran.1.1.1.2 = i) -> ∃ tran', trans' !! h = Some tran' ∧ tran = tran') trans.
-
-  Definition slice_wf (Φ: (gmap Addr transaction) -> VMID -> VMID -> iProp Σ) :=
-    ∀ i j trans trans', trans_preserve_slice i j trans trans'->
-    (Φ trans i j ⊣⊢ Φ trans' i j).
-
-  Definition slice_wf2 (Φ: (gmap Addr transaction) -> VMID -> VMID -> iProp Σ) :=
-    ∀ i j (trans trans' : gmap Addr transaction),
-    dom (gset _) (filter (λ kv, kv.2.1.1.1.1 = i ∧ kv.2.1.1.1.2 = j)%type trans') ⊆ dom _ trans ->
-    ([∗ map] h ↦ tran ∈ trans, h -{1/2}>t tran.1) ⊢
-    (Φ trans' i j) ∗-∗ (Φ (map_zip (fst<$>trans) (snd <$>trans')) i j).
-
-  Class SliceWf (Φ: (gmap Addr transaction) -> VMID -> VMID-> iProp Σ):=
-    {
-      slice : (slice_wf Φ);
-      agree : (slice_wf2 Φ)
-    }.
-
-  Program Definition interp_access_prim Φ p_tx p_rx ps_acc trans `(!SliceWf Φ): iPropO Σ:=
+  Program Definition interp_access_prim Φ p_tx p_rx ps_acc trans `{!SliceWf Φ}: iPropO Σ:=
     (
-      (* let ps_macc_trans := (transferred_memory_pages_all trans) in *)
+      (* making sure we have enough resources for V0 *)
+      ⌜∀ i j trans, (i = V0 ∨ j = V0) -> Φ trans i j ⊣⊢ slice_transfer_all trans i j⌝ ∗
       let ps_oea := ps_acc ∖ {[p_rx;p_tx]} ∖ (currently_accessible_in_trans_memory_pages V0 trans) in
       (∃ regs, ⌜is_total_gmap regs⌝ ∗ [∗ map] r ↦ w ∈ regs, r @@ V0 ->r w) ∗
       (tx_page V0 p_tx ∗ ∃ mem_tx, memory_page p_tx mem_tx) ∗
@@ -75,10 +181,7 @@ Section logrel_prim.
       transaction_hpool_global_transferred trans ∗
       rx_pages (list_to_set (list_of_vmids) ∖ {[V0]}) ∗
       (big_sepSS set_of_vmids (Φ trans)) ∗
-      (* transaction_pagetable_entries_transferred_all trans ∗ *)
-      (* retrievable_transaction_transferred_all trans ∗ *)
-      (* (∃ mem_trans, memory_pages ps_macc_trans mem_trans) ∗ *)
-      [∗ set] i ∈ set_of_vmids ∖ {[V0]}, VMProp (i:VMID) (vmprop_unknown i p_tx p_rx) (1/2)%Qp
+      [∗ set] i ∈ set_of_vmids ∖ {[V0]}, VMProp (i:VMID) (vmprop_unknown i Φ p_tx p_rx) (1/2)%Qp
     )%I.
 
 End logrel_prim.
